start to separate prop and program atoms in Vocab

Pdl/Vocab.lean
@@ -2,36 +2,77 @@ import Pdl.Syntax
 
 import Mathlib.Data.Finset.Basic
 import Mathlib.Data.Finset.Union
+import Mathlib.Data.Finset.Fold
+
+/-- A vocabulary is a pair of
+    1. a set of atomic propositions and
+    2. a set of atomic programs. -/
+structure Vocab where
+  props : Finset Nat
+  progs : Finset Nat
+deriving DecidableEq
+
+@[simp]
+def Vocab.union (a : Vocab) (b : Vocab) : Vocab := ⟨a.1 ∪ b.1, a.2 ∪ b.2⟩
+
+instance : Std.Commutative Vocab.union := sorry
+
+instance : Std.Associative Vocab.union := sorry
+
+instance : Union Vocab := ⟨Vocab.union⟩
+
+@[simp]
+instance : EmptyCollection Vocab := ⟨ ⟨{}, {}⟩ ⟩
+
+@[simp]
+instance : Membership ℕ Vocab := ⟨fun n v => n ∈ v.1 ∨ n ∈ v.2⟩
+
+@[simp]
+def Vocab.fromList (l : List Vocab) : Vocab := l.foldr (.union) {}
+
+@[simp]
+def Vocab.fromFinset (X : Finset Vocab) : Vocab := X.fold (Vocab.union) {} id
 
 mutual
-  def vocabOfProgram : Program → Finset Nat
-    | ·c => {c}
+  def vocabOfProgram : Program → Vocab
+    | ·c => ⟨{c}, {}⟩
     | α;'β => vocabOfProgram α ∪ vocabOfProgram β
     | α ⋓ β => vocabOfProgram α ∪ vocabOfProgram β
     | ∗α => vocabOfProgram α
     | ?' φ => vocabOfFormula φ
-  def vocabOfFormula : Formula → Finset Nat
-    | ⊥ => ∅
-    | ·c => {c}
+  def vocabOfFormula : Formula → Vocab
+    | ⊥ => {}
+    | ·c => ⟨{c}, {}⟩
     | ~φ => vocabOfFormula φ
     | φ⋀ψ => vocabOfFormula φ ∪ vocabOfFormula ψ
     | ⌈α⌉ φ => vocabOfProgram α ∪ vocabOfFormula φ
 end
 
-def vocabOfSetFormula : Finset Formula → Finset Nat
-  | X => X.biUnion vocabOfFormula
+@[simp]
+theorem Vocab.props_dist {X Y : Vocab} : (X ∪ Y).props = X.props ∪ Y.props := by sorry
 
-def vocabOfListFormula : List Formula → Finset Nat
-  | X => (X.toFinset).biUnion vocabOfFormula
+@[simp]
+theorem Vocab.progs_dist {X Y : Vocab} : (X ∪ Y).progs = X.progs ∪ Y.progs := by sorry
 
-def vocabOfListProgram : List Program → Finset Nat
-  | X => (X.toFinset).biUnion vocabOfProgram
+def vocabOfSetFormula : Finset Formula → Vocab
+  | X => .fromFinset (X.biUnion (fun f => {vocabOfFormula f}))
 
-theorem inVocList : ℓ ∈ vocabOfListFormula L ↔ ∃φ ∈ L, ℓ ∈ vocabOfFormula φ := by
-  simp only [vocabOfListFormula, Finset.mem_biUnion, List.mem_toFinset]
+def vocabOfListFormula : List Formula → Vocab
+  | X => .fromList (X.map vocabOfFormula)
+
+def vocabOfListProgram : List Program → Vocab
+  | X => .fromList (X.map vocabOfProgram)
+
+@[simp]
+theorem inVocList : n ∈ vocabOfListFormula L ↔ ∃φ ∈ L, n ∈ vocabOfFormula φ := by
+  induction L
+  · simp [vocabOfListFormula]
+  case cons φ L IH =>
+    cases em (n ∈ vocabOfFormula φ) <;> simp_all [vocabOfListFormula]
+    sorry
 
 class HasVocabulary (α : Type) where
-  voc : α → Finset Nat
+  voc : α → Vocab
 
 instance formulaHasVocabulary : HasVocabulary Formula := ⟨vocabOfFormula⟩
 instance programHasVocabulary : HasVocabulary Program := ⟨vocabOfProgram⟩
